examples/sess/trusted.v
@@ -160,7 +160,7 @@ Lemma trusted_wp_connect N p c skI skR :
   {{{ True }}}
     Sess.connect c skI (Spec.pkey skR) (Tag N)
   {{{ cs, RET (repr cs);
-      trusted_connected skI skR Init cs p }}}.
+      trusted_connected skI skR Init cs (p skI skR cs) }}}.
 Proof.
 iIntros "#chan #ctx #sess #m_skI #m_skR #hon_I #hon_R".
 iIntros "%Φ !> pre post".
@@ -194,11 +194,10 @@ Lemma trusted_wp_confirm N p c skI skR ga :
   minted skR -∗
   □ (public skI → ▷ False) -∗
   □ (public skR → ▷ False) -∗
-  {{{ public ga ∗ minted skI ∗ minted skR 
-       }}}
+  {{{ public ga ∗ minted skI ∗ minted skR }}}
     Sess.confirm c skR (Tag N) (ga, Spec.pkey skI)%V
   {{{ cs, RET (repr cs);
-      trusted_connected skI skR Resp cs (iProto_dual p) }}}.
+      trusted_connected skI skR Resp cs (iProto_dual (p skI skR cs)) }}}.
 Proof.
 iIntros "#chan #ctx #sess #m_skI #m_skR #hon_I #hon_R".
 iIntros "%Φ !> (#p_ga & #m_skI' & #m_skR') post".
@@ -207,7 +206,8 @@ wp_lam; wp_pures. iApply wp_fupd.
 wp_apply (GenConn.wp_confirm True with "[]").
 - eauto.
 - iFrame "#". iSplit; last iRight => //. iIntros "!> %b tok".
-  iMod (iProto_init p) as (γl γr) "(proto_ctx & ownI & ownR)".
+  set si := SessInfo _ _ _ _ _.
+  iMod (iProto_init (p skI skR si)) as (γl γr) "(proto_ctx & ownI & ownR)".
   iMod (term_meta_set (sessN.@"names") (γl, γr) with "tok") as "#meta".
   { solve_ndisj. }
   iModIntro. iSplitL "ownI". { iExists (γl, γr). iFrame. by eauto. }
